WIP refactoring Wasm_Properties.thy: halfway through.

WebAssembly/Wasm.thy
@@ -196,8 +196,8 @@ inductive reduce_simple :: "[e list, e list] \<Rightarrow> bool" ("\<lparr>_\<rp
   \<comment> \<open>\<open>drop\<close>\<close>
 | drop:"\<lparr>[$C v, ($ Drop)]\<rparr> \<leadsto> \<lparr>[]\<rparr>"
   \<comment> \<open>\<open>select\<close>\<close>
-| select_false:"int_eq n 0 \<Longrightarrow> \<lparr>[$C v1, $C v2, $EConstNum (ConstInt32 n), ($ Select)]\<rparr> \<leadsto> \<lparr>[$(C v2)]\<rparr>"
-| select_true:"int_ne n 0 \<Longrightarrow> \<lparr>[$C v1, $C v2, $EConstNum (ConstInt32 n), ($ Select)]\<rparr> \<leadsto> \<lparr>[$(C v1)]\<rparr>"
+| select_false:"int_eq n 0 \<Longrightarrow> \<lparr>[$C v1, $C v2, $EConstNum (ConstInt32 n), ($ Select)]\<rparr> \<leadsto> \<lparr>[$C v2]\<rparr>"
+| select_true:"int_ne n 0 \<Longrightarrow> \<lparr>[$C v1, $C v2, $EConstNum (ConstInt32 n), ($ Select)]\<rparr> \<leadsto> \<lparr>[$C v1]\<rparr>"
   \<comment> \<open>\<open>if\<close>\<close>
 | if_false:"int_eq n 0 \<Longrightarrow> \<lparr>[$EConstNum (ConstInt32 n), $(If tb e1s e2s)]\<rparr> \<leadsto> \<lparr>[$(Block tb e2s)]\<rparr>"
 | if_true:"int_ne n 0 \<Longrightarrow> \<lparr>[$EConstNum (ConstInt32 n), $(If tb e1s e2s)]\<rparr> \<leadsto> \<lparr>[$(Block tb e1s)]\<rparr>"
@@ -236,11 +236,11 @@ inductive reduce :: "[s, f, e list, s, f, e list] \<Rightarrow> bool" ("\<lparr>
 | invoke_host_Some:"\<lbrakk>(funcs s!i_cl) = Func_host (t1s _> t2s) h; ves = ($C* vcs); length vcs = n; length t1s = n; length t2s = m; host_apply s (t1s _> t2s) h vcs hs (Some (s', vcs'))\<rbrakk> \<Longrightarrow> \<lparr>s;f;ves @ [Invoke i_cl]\<rparr> \<leadsto> \<lparr>s';f;($C* vcs')\<rparr>"
 | invoke_host_None:"\<lbrakk>(funcs s!i_cl) = Func_host (t1s _> t2s) h; ves = ($C* vcs); length vcs = n; length t1s = n; length t2s = m\<rbrakk> \<Longrightarrow> \<lparr>s;f;ves @ [Invoke i_cl]\<rparr> \<leadsto> \<lparr>s;f;[Trap]\<rparr>"
   \<comment> \<open>\<open>get_local\<close>\<close>
-| get_local:"\<lbrakk>length vi = j; f_locs f = (vi @ [v] @ vs)\<rbrakk> \<Longrightarrow> \<lparr>s;f;[$(Get_local j)]\<rparr> \<leadsto> \<lparr>s;f;[$(C v)]\<rparr>"
+| get_local:"\<lbrakk>length vi = j; f_locs f = (vi @ [v] @ vs)\<rbrakk> \<Longrightarrow> \<lparr>s;f;[$(Get_local j)]\<rparr> \<leadsto> \<lparr>s;f;[$C v]\<rparr>"
   \<comment> \<open>\<open>set_local\<close>\<close>
-| set_local:"\<lbrakk>length vi = j\<rbrakk> \<Longrightarrow> \<lparr>s;\<lparr> f_locs = (vi @ [v] @ vs), f_inst = i \<rparr>;[$(C v'), $(Set_local j)]\<rparr> \<leadsto> \<lparr>s;\<lparr> f_locs = (vi @ [v'] @ vs), f_inst = i \<rparr>;[]\<rparr>"
+| set_local:"\<lbrakk>length vi = j\<rbrakk> \<Longrightarrow> \<lparr>s;\<lparr> f_locs = (vi @ [v] @ vs), f_inst = i \<rparr>;[$C v', $(Set_local j)]\<rparr> \<leadsto> \<lparr>s;\<lparr> f_locs = (vi @ [v'] @ vs), f_inst = i \<rparr>;[]\<rparr>"
   \<comment> \<open>\<open>get_global\<close>\<close>
-| get_global:"\<lparr>s;f;[$(Get_global j)]\<rparr> \<leadsto> \<lparr>s;f;[$ C(sglob_val s (f_inst f) j)]\<rparr>"
+| get_global:"\<lparr>s;f;[$(Get_global j)]\<rparr> \<leadsto> \<lparr>s;f;[$C(sglob_val s (f_inst f) j)]\<rparr>"
   \<comment> \<open>\<open>set_global\<close>\<close>
 | set_global:"supdate_glob s (f_inst f) j v = s' \<Longrightarrow> \<lparr>s;f;[$C v, $(Set_global j)]\<rparr> \<leadsto> \<lparr>s';f;[]\<rparr>"
   \<comment> \<open>\<open>load\<close>\<close>
